@base <http://w3id.org/oseg/ont/okhmeta> .
@prefix cc: <http://creativecommons.org/ns#> .
@prefix dcam: <http://purl.org/dc/dcam/> .
@prefix dcat: <http://www.w3.org/ns/dcat#> .
@prefix dcterms: <http://purl.org/dc/terms/> .
@prefix okhmeta: <http://w3id.org/oseg/ont/okhmeta#> .
@prefix osegprof: <http://w3id.org/oseg/ont/oseg-profiles#> .
@prefix owl: <http://www.w3.org/2002/07/owl#> .
@prefix rdf: <http://www.w3.org/1999/02/22-rdf-syntax-ns#> .
@prefix rdfs: <http://www.w3.org/2000/01/rdf-schema#> .
@prefix schema: <http://schema.org/> .
@prefix skos: <http://www.w3.org/2004/02/skos/core#> .
@prefix spdx: <http://spdx.org/rdf/terms#> .
@prefix spdxl: <http://spdx.org/licenses/> .
@prefix vaem: <http://www.linkedmodel.org/schema/vaem#> .
@prefix vann: <http://purl.org/vocab/vann/> .
@prefix vs: <http://www.w3.org/2003/06/sw-vocab-status/ns#> .
@prefix xsd: <http://www.w3.org/2001/XMLSchema#> .

<>
  a
    owl:Ontology ,
    spdx:SpdxItem ;
  rdfs:comment """
# SPDX-FileCopyrightText: 2024 Robin Vobruba <hoijui.quaero@gmail.com>
#
# SPDX-License-Identifier: GPL-3.0-or-later
""" ;
  owl:versionInfo "1.1.0" ;
  owl:versionIRI <http://w3id.org/oseg/ont/1.1.0/okh-meta> ;
  cc:license "https://www.gnu.org/licenses/gpl-3.0.txt" ;
  dcat:contactPoint "https://github.com/iop-alliance/OpenKnowHow/" ;
  dcat:keyword
    "OKH" ,
    "grouping" ,
    "meta" ,
    "tagging" ;
  dcterms:created "2024-07-01"^^xsd:date ;
  dcterms:creator osegprof:robinVobruba ;
  dcterms:description """Used for tagging/grouping classes and properties in the OKH ontology.
This hopefully allows to filter and visualize only (relevant) parts
of the ontology/data,
given specific scenarios.
For example,
one could only show the classes and properties tagged with "basic",
when browsing multiple projects at a time."""@en ;
  dcterms:issued "2024-07-01T09:03:49Z"^^xsd:dateTimeStamp ;
  dcterms:language <http://id.loc.gov/vocabulary/iso639-1/en> ;
  dcterms:license "https://www.gnu.org/licenses/gpl-3.0.txt" ;
  dcterms:publisher osegprof:Iopa ;
  dcterms:source "https://github.com/iop-alliance/OpenKnowHow/master/src/spec/okh-meta.ttl" ;
  dcterms:title "Open Know How (OKH) - Meta"@en ;
  schema:codeRepository "https://github.com/iop-alliance/OpenKnowHow/" ;
  schema:creator osegprof:robinVobruba ;
  skos:editorialNote """Regarding the use of `dcam:domainIncludes`
and `dcam:rangeIncludes` in this ontology:
Looking at the definitions for the RDFS version
of the two, `rdfs:domain` and `rdfs:range`:
* https://www.w3.org/TR/rdf-schema/#ch_domain
* https://www.w3.org/TR/rdf-schema/#ch_range
and as described in this StackOverflow answer:
<https://stackoverflow.com/a/74782257/586229>,
multiple objects for the two RDFS properties mean,
that *all of them* apply, simultaneously,
not *one of them*.
You may think of this as an `AND` coupling.
We want the *one of them* meaning though (`OR`).
The `dcam:*` properties give us just that.
Though there is an additional,
very important difference:
The `*Includes` properties are just suggestions,
so if they are used, it is left open to use other,
not mentioned class as domain or range too."""@en ;
  spdx:licenseDeclared spdxl:GPL-3.0-or-later ;
  vann:preferredNamespacePrefix "okhmeta" ;
  vann:preferredNamespaceUri "http://w3id.org/oseg/ont/okh-meta#" ;
  .

okhmeta:Tag
  a
    owl:Class ,
    skos:Concept ;
  rdfs:label "meta tag"@en ;
  rdfs:comment "see property okhmeta:hasMetaTag"@en ;
  rdfs:subClassOf skos:Collection ;
  vs:term_status "unstable" ;
  okhmeta:hasMetaTag okhmeta:MetaTag ;
  .

okhmeta:hasMetaTag
  a
    owl:ObjectProperty ,
    skos:Concept ;
  rdfs:label "has meta tag"@en ;
  rdfs:comment """Tags any part of the ontology with a meta-tag.
This might be useful for arranging properties in a GUI,
or for visualizing only parts of the ontology in a graph,
among possibly other things."""@en ;
  rdfs:subPropertyOf skos:member ;
  dcam:rangeIncludes okhmeta:MetaTag ;
  vs:term_status "unstable" ;
  okhmeta:hasMetaTag okhmeta:MetaTag ;
  .

okhmeta:AcademicTag
  a okhmeta:Tag ;
  rdfs:label "academic"@en ;
  rdfs:comment "The annotated subject is primarily interesting in the academic context"@en ;
  vs:term_status "unstable" ;
  okhmeta:hasMetaTag okhmeta:MetaTag ;
  .

okhmeta:BasicTag
  a okhmeta:Tag ;
  rdfs:label "basic"@en ;
  rdfs:comment "The annotated subject is a member of the basic-description-part of a project"@en ;
  vs:term_status "unstable" ;
  okhmeta:hasMetaTag okhmeta:MetaTag ;
  .

okhmeta:DataGatheringTag
  a okhmeta:Tag ;
  rdfs:label "data gathering"@en ;
  rdfs:comment "The annotated subject deals with meta-data about the OKH data-gathering process"@en ;
  vs:term_status "unstable" ;
  okhmeta:hasMetaTag okhmeta:MetaTag ;
  .

okhmeta:DataTag
  a okhmeta:Tag ;
  rdfs:label "data"@en ;
  rdfs:comment "The annotated subject is interesting when gathering data of the project"@en ;
  vs:term_status "unstable" ;
  okhmeta:hasMetaTag okhmeta:MetaTag ;
  .

okhmeta:DevelopmentTag
  a okhmeta:Tag ;
  rdfs:label "development"@en ;
  rdfs:comment "The annotated subject is a member of the development-/design-part of a project"@en ;
  vs:term_status "unstable" ;
  okhmeta:hasMetaTag okhmeta:MetaTag ;
  .

okhmeta:DocumentationTag
  a okhmeta:Tag ;
  rdfs:label "documentation"@en ;
  rdfs:comment "The annotated subject is a member of the documentation-part of a project"@en ;
  vs:term_status "unstable" ;
  okhmeta:hasMetaTag okhmeta:MetaTag ;
  .

okhmeta:ExtendedInfoTag
  a okhmeta:Tag ;
  rdfs:label "extended info"@en ;
  rdfs:comment "The annotated subject deals with extended info about a project. This is somewhat the opposite of the 'basic' tag. The idea is, that there is third set of OKH parts, that lay inbetween these two extremes, and are not tagged with a specific, third tag."@en ;
  vs:term_status "unstable" ;
  okhmeta:hasMetaTag okhmeta:MetaTag ;
  .

okhmeta:HistoryTag
  a okhmeta:Tag ;
  rdfs:label "history info"@en ;
  rdfs:comment "The annotated subject deals with the projects history."@en ;
  vs:term_status "unstable" ;
  okhmeta:hasMetaTag okhmeta:MetaTag ;
  .

okhmeta:IdentificationTag
  a okhmeta:Tag ;
  rdfs:label "identification"@en ;
  rdfs:comment "The annotated subject can be used to identify the project (potentially in combination with other identity narrowing subjects)."@en ;
  vs:term_status "unstable" ;
  okhmeta:hasMetaTag okhmeta:MetaTag ;
  .

okhmeta:LegalTag
  a okhmeta:Tag ;
  rdfs:label "legal"@en ;
  rdfs:comment "The annotated subject deals with legal issues about the project. This will be things like the licensor(s), the license(s), and disclaimers."@en ;
  vs:term_status "unstable" ;
  okhmeta:hasMetaTag okhmeta:MetaTag ;
  .

okhmeta:MakingTag
  a okhmeta:Tag ;
  rdfs:label "making"@en ;
  rdfs:comment "The annotated subject deals with the creation of the actual hardware. This includes (at least) manufacturing and assembly related issues, plus the documentation for these steps."@en ;
  vs:term_status "unstable" ;
  okhmeta:hasMetaTag okhmeta:MetaTag ;
  .

okhmeta:MetaTag
  a okhmeta:Tag ;
  rdfs:label "meta"@en ;
  rdfs:comment "The annotated subject is a member of the meta-part of the ontology"@en ;
  vs:term_status "unstable" ;
  okhmeta:hasMetaTag okhmeta:MetaTag ;
  .

okhmeta:PartsTag
  a okhmeta:Tag ;
  rdfs:label "parts"@en ;
  rdfs:comment "The annotated subject deals with sub-parts and the modular nature of a project."@en ;
  vs:term_status "unstable" ;
  okhmeta:hasMetaTag okhmeta:MetaTag ;
  .

okhmeta:PhysicalTag
  a okhmeta:Tag ;
  rdfs:label "physical"@en ;
  rdfs:comment "The annotated subject deals with properties about the physical product(s) of the project."@en ;
  vs:term_status "unstable" ;
  okhmeta:hasMetaTag okhmeta:MetaTag ;
  .

okhmeta:QualityTag
  a okhmeta:Tag ;
  rdfs:label "quality"@en ;
  rdfs:comment "The annotated subject deals with quality indication (and later also assurance), both of the documentation and the physical product(s) of the project."@en ;
  vs:term_status "unstable" ;
  okhmeta:hasMetaTag okhmeta:MetaTag ;
  vaem:todo "TODO Should this really be both about the docu and the physical project?"@en ;
  .

okhmeta:TransportationTag
  a okhmeta:Tag ;
  rdfs:label "transportation"@en ;
  rdfs:comment "The annotated subject matters for transporting the physical product(s) of the project."@en ;
  vs:term_status "unstable" ;
  okhmeta:hasMetaTag okhmeta:MetaTag ;
  .
