@base <http://w3id.org/oseg/ont/okh> .
@prefix cc: <http://creativecommons.org/ns#> .
@prefix dcam: <http://purl.org/dc/dcam/> .
@prefix dcat: <http://www.w3.org/ns/dcat#> .
@prefix dcterms: <http://purl.org/dc/terms/> .
@prefix dctype: <http://purl.org/dc/dcmitype/> .
@prefix foaf: <http://xmlns.com/foaf/0.1/> .
@prefix mime: <http://www.iana.org/assignments/media-types/> .
@prefix npg: <http://ns.nature.com/terms/> .
@prefix obo: <http://purl.obolibrary.org/obo/> .
@prefix ods: <http://w3id.org/oseg/ont/ods#> .
@prefix okh: <http://w3id.org/oseg/ont/okh#> .
@prefix okhimg: <http://w3id.org/oseg/ont/okhimg#> .
@prefix okhkrawl: <http://w3id.org/oseg/ont/okh-krawler#> .
@prefix okhmeta: <http://w3id.org/oseg/ont/okhmeta#> .
@prefix osegprof: <http://w3id.org/oseg/ont/oseg-profiles#> .
@prefix otrl: <http://w3id.org/oseg/ont/otrl#> .
@prefix owl: <http://www.w3.org/2002/07/owl#> .
@prefix patent: <http://data.epo.org/linked-data/def/patent/> .
@prefix rdf: <http://www.w3.org/1999/02/22-rdf-syntax-ns#> .
@prefix rdfs: <http://www.w3.org/2000/01/rdf-schema#> .
@prefix schema: <http://schema.org/> .
@prefix sh: <http://www.w3.org/ns/shacl#> .
@prefix skos: <http://www.w3.org/2004/02/skos/core#> .
@prefix spdx: <http://spdx.org/rdf/terms#> .
@prefix spdxl: <http://spdx.org/licenses/> .
@prefix tsdc: <http://w3id.org/oseg/ont/tsdc/core#> .
@prefix vaem: <http://www.linkedmodel.org/schema/vaem#> .
@prefix vann: <http://purl.org/vocab/vann/> .
@prefix void: <http://rdfs.org/ns/void#> .
@prefix vs: <http://www.w3.org/2003/06/sw-vocab-status/ns#> .
@prefix xsd: <http://www.w3.org/2001/XMLSchema#> .

<>
  a
    dcterms:Standard ,
    owl:Ontology ,
    spdx:SpdxItem ;
  owl:versionInfo "1.1.0" ;
  owl:versionIRI <http://w3id.org/oseg/ont/1.1.0/okh> ;
  cc:license "https://www.gnu.org/licenses/gpl-3.0.txt"^^xsd:anyURI ;
  dcat:contactPoint "https://github.com/iop-alliance/OpenKnowHow/issues/"^^xsd:anyURI ;
  dcat:keyword
    "OKH" ,
    "design" ,
    "hardware" ,
    "open-source" ,
    "open-source-hardware" ,
    "project" ;
  dcterms:created "2020-10-02Z"^^xsd:date ;
  dcterms:creator
    osegprof:martinHaeuer ,
    osegprof:robinVobruba ;
  dcterms:description "Used for indexing, searching and comparing Open Source Hardware projects"@en ;
  dcterms:issued "2021-08-24T16:32:33Z"^^xsd:dateTimeStamp ;
  dcterms:language <http://id.loc.gov/vocabulary/iso639-1/en> ;
  dcterms:license "https://www.gnu.org/licenses/gpl-3.0.txt"^^xsd:anyURI ;
  dcterms:modified "2022-02-22T12:01:28Z"^^xsd:dateTimeStamp ;
  dcterms:publisher osegprof:Iopa ;
  dcterms:source "https://github.com/iop-alliance/OpenKnowHow/master/src/spec/okh.ttl"^^xsd:anyURI ;
  dcterms:title "Open Know How (OKH) ontology"@en ;
  schema:codeRepository "https://github.com/iop-alliance/OpenKnowHow/"^^xsd:anyURI ;
  schema:creator
    osegprof:martinHaeuer ,
    osegprof:robinVobruba ;
  sh:declare
    [
      sh:namespace "https://w3id.org/oseg/ont/okh#"^^xsd:anyURI ;
      sh:prefix "okh" ;
    ] ;
  sh:suggestedShapesGraph <https://w3id.org/oseg/ont/okh/shacl#Ontology> ;
  skos:editorialNote
    """Regarding the use of `dcam:domainIncludes`
and `dcam:rangeIncludes` in this ontology:
Looking at the definitions for the RDFS version
of the two, `rdfs:domain` and `rdfs:range`:
* https://www.w3.org/TR/rdf-schema/#ch_domain
* https://www.w3.org/TR/rdf-schema/#ch_range
and as described in this StackOverflow answer:
<https://stackoverflow.com/a/74782257/586229>,
multiple objects for the two RDFS properties mean,
that *all of them* apply, simultaneously,
not *one of them*.
You may think of this as an `AND` coupling.
We want the *one of them* meaning though (`OR`).
The `dcam:*` properties give us just that.
Though there is an additional,
very important difference:
The `*Includes` properties are just suggestions,
so if they are used, it is left open to use other,
not mentioned class as domain or range too."""@en ,
    """
# SPDX-FileCopyrightText: 2020 - 2021 Martin Häuer <martin.haeuer@ose-germany.de>
# SPDX-FileCopyrightText: 2020 - 2025 Robin Vobruba <hoijui.quaero@gmail.com>
#
# SPDX-License-Identifier: GPL-3.0-or-later
""" ,
    """# Naming Convention

- Classes:

   Guideline:

   - in Upper[CamelCase]
   - a single noun or multiple, combined nouns

   Examples:

   - `ex:Person`
   - `ex:InfillHose`

- Datatypes:

   Guideline:

   - in lower[CamelCase]
   - a single noun or multiple, combined nouns

   Examples:

   - `ex:float`
   - `ex:emailString`

- Predicates:

   - in lower[CamelCase]
   - if a DatatypeProperty,
      i.e. one with a literal as range/object,
      it should be a noun (or a combined noun)
   - if an (Object)Property,
     i.e. a relation between non-literals),
     it should be a verb plus potentially a noun (potentially combined),
     though an initial 'is' should be omitted.

   Examples:

   - `ex:age 55`
   - `ex:enrolled true`
   - `ex:depicts "A plant with a purple flower"@en`
   - `ex:hasMother ex:albaBach`
   - `ex:olderThen ex:albaBach`
   - `ex:likes ex:albaBach`

- Individuals:
   - in lower[CamelCase]
   - a single noun or multiple, combined nouns

   Examples:

   - `ex:albaBach`
   - `ex:paris`

See our [naming convention issue](
https://github.com/iop-alliance/OpenKnowHow/issues/13)
for more details.

[CamelCase]: https://en.wikipedia.org/wiki/Camel_case
""" ,
    """We try to follow:
(Recommendations for Vocabulary_Design](
https://lov.linkeddata.es/Recommendations_Vocabulary_Design.pdf)""" ,
    """We try to follow:
[Semantic Web and Linked Data: Best Practices and Standards](
https://guides.library.ucla.edu/semantic-web/bestpractices#s-lg-page-section-2410777)""" ;
  spdx:licenseDeclared spdxl:GPL-3.0-or-later ;
  vann:preferredNamespacePrefix "okh" ;
  vann:preferredNamespaceUri "http://w3id.org/oseg/ont/okh#"^^xsd:anyURI ;
  void:rootResource
    okh:Module ,
    okh:Part ;
  .

okh:Component
  a
    owl:Class ,
    skos:Concept ;
  rdfs:label "component"@en ;
  rdfs:comment "Either a module (MOSH) or Part (POSH); more component types may be added in the future"@en ;
  vs:term_status "unstable" ;
  okhmeta:hasMetaTag okhmeta:PartsTag ;
  vaem:todo "TODO `rdfs:subClassOf schema:CreativeWork ;`? - Probably better suited for the OSH Ontology -- `rdfs:subClassOf schema:CreativeWork ;`?" ;
  .

okh:Dimensions
  a
    owl:Class ,
    skos:Concept ;
  rdfs:label "outer dimensions"@en ;
  rdfs:comment """… of a module or a part;
This follows the same logic as the "bounding-box" in computer graphics,
but in the physical world.
This is commonly used to calculate (or at least estimate)
how many items of a manufactured module or part
can be packed into storage space of known dimensions."""@en ;
  rdfs:subClassOf dcterms:SizeOrDuration ;
  vs:term_status "unstable" ;
  okhmeta:hasMetaTag
    okhmeta:PhysicalTag ,
    okhmeta:TransportationTag ;
  .

okh:Image
  a
    owl:Class ,
    skos:Concept ;
  rdfs:label "image"@en ;
  rdfs:subClassOf
    dctype:StillImage ,
    foaf:Image ,
    ods:File ,
    schema:ImageObject ;
  vs:term_status "unstable" ;
  okhmeta:hasMetaTag okhmeta:BasicTag ;
  .

okh:ManifestFile
  a
    owl:Class ,
    skos:Concept ;
  rdfs:label "manifest file"@en ;
  rdfs:comment "source file holding this projects OKH data in TOML format, from which RDF is generated"@en ;
  rdfs:subClassOf
    ods:File ,
    schema:TextDigitalDocument ;
  vs:term_status "unstable" ;
  okhmeta:hasMetaTag okhmeta:DataGatheringTag ;
  vaem:todo "TODO Comment out/remove this subject - This is now ODS territory, though there we use an ods:File now" ;
  .

okh:Module
  a
    owl:Class ,
    skos:Concept ;
  rdfs:label "module"@en ;
  rdfs:comment "Module of Open Source Hardware (MOSH)"@en ;
  rdfs:subClassOf okh:Component ;
  vs:term_status "unstable" ;
  okhmeta:hasMetaTag okhmeta:PartsTag ;
  .

okh:Part
  a
    owl:Class ,
    skos:Concept ;
  rdfs:label "part"@en ;
  rdfs:comment "Piece of Open Source Hardware (POSH)"@en ;
  rdfs:subClassOf okh:Component ;
  vs:term_status "unstable" ;
  okhmeta:hasMetaTag okhmeta:PartsTag ;
  .

okh:Publication
  a
    owl:Class ,
    skos:Concept ;
  rdfs:label "scientific publication"@en ;
  rdfs:comment "_scientific_ (that is: peer reviewed) publication that _contains_ the design files"@en ;
  rdfs:subClassOf npg:Publication ;
  vs:term_status "unstable" ;
  okhmeta:hasMetaTag
    okhmeta:AcademicTag ,
    okhmeta:QualityTag ;
  .

okh:Software
  a
    owl:Class ,
    skos:Concept ;
  rdfs:label "software"@en ;
  rdfs:comment "Software (including firmware) needed to run & use the OSH"@en ;
  rdfs:subClassOf
    dctype:Software ,
    okh:Component ;
  vs:term_status "unstable" ;
  okhmeta:hasMetaTag okhmeta:PartsTag ;
  .

okh:Standard
  a
    owl:Class ,
    skos:Concept ;
  rdfs:label "technical standard"@en ;
  rdfs:comment "official standard used in the _design_ (_not_ e.g. DIN SPEC 3105-1)"@en ;
  rdfs:subClassOf dcterms:Standard ;
  vs:term_status "unstable" ;
  okhmeta:hasMetaTag okhmeta:QualityTag ;
  vaem:todo "TODO We need a list of individuals of this class somewhere. It should already exist out there!" ;
  .

okh:compliesWith
  a
    owl:ObjectProperty ,
    skos:Concept ;
  rdfs:label "complies with"@en ;
  rdfs:comment "Links to a standard the subject complies with"@en ;
  rdfs:subPropertyOf dcterms:conformsTo ;
  dcam:domainIncludes okh:Component ;
  dcam:rangeIncludes okh:Standard ;
  vs:term_status "unstable" ;
  okhmeta:hasMetaTag okhmeta:QualityTag ;
  .

okh:documentationReadinessLevel
  a
    owl:ObjectProperty ,
    skos:Concept ;
  rdfs:label "Documentation Readiness Level (DLR)"@en ;
  rdfs:comment "Indicates the development stage of the **documentation** using the ODRL definitions; see the OTRL ontology."@en ;
  dcam:domainIncludes okh:Module ;
  dcam:rangeIncludes otrl:ODRL ;
  vs:term_status "unstable" ;
  owl:maxCardinality 1 ;
  okhmeta:hasMetaTag
    okhmeta:DevelopmentTag ,
    okhmeta:QualityTag ;
  skos:example
    otrl:ODRL1 ,
    otrl:ODRL2 ,
    otrl:ODRL3 ,
    otrl:ODRL3Star ,
    otrl:ODRL4 ;
  .

okh:fillsSlot
  a
    owl:ObjectProperty ,
    skos:Concept ;
  rdfs:label "fills slot"@en ;
  rdfs:comment """Denotes the slot the image fills within the subject it belongs to.
You may also think of it as the 'role' the image plays for its parent.
The available slots are predefined,
see the [OKH image slots](http://w3id.org/oseg/ont/okhimg#slots);
there you will also read about the ability to define custom ones,
though you might also consider proposing a new common tag
[in an issue](https://github.com/iop-alliance/OpenKnowHow/issues/new).
An image can fill multiple slots,
but each slot can be filled at most once.
This is useful for things like the projects icon,
or the left-side view of the 3D model."""@en ;
  rdfs:subPropertyOf schema:keywords ;
  dcam:domainIncludes okh:Image ;
  dcam:rangeIncludes xsd:string ;
  vs:term_status "unstable" ;
  skos:example okhimg:slotIconMain ;
  .

okh:forkOf
  a
    owl:ObjectProperty ,
    skos:Concept ;
  rdfs:label "fork of"@en ;
  rdfs:comment "Indicates that this project was split of (aka forked) from an other project at some point in the past"@en ;
  rdfs:subPropertyOf schema:isBasedOn ;
  dcam:domainIncludes okh:Component ;
  dcam:rangeIncludes okh:Component ;
  vs:term_status "unstable" ;
  owl:maxCardinality 1 ;
  okhmeta:hasMetaTag
    okhmeta:HistoryTag ,
    okhmeta:IdentificationTag ;
  .

okh:hasAuxiliary
  a
    owl:ObjectProperty ,
    skos:Concept ;
  rdfs:label "has auxiliary file"@en ;
  rdfs:comment "This links to files associated with the subject, which classify neither as source nor as export, but are still useful in the repository"@en ;
  dcam:domainIncludes okh:Component ;
  dcam:rangeIncludes ods:File ;
  rdfs:seeAlso
    okh:hasExport ,
    okh:hasSource ;
  vs:term_status "unstable" ;
  okhmeta:hasMetaTag okhmeta:DataTag ;
  skos:example
    "https://file-hosting-service.org/accounts/my_project/res/media/img/project_logo.svg" ,
    "kicad_libs/cool_3rd_party_parts.lib" ,
    "res/media/img/project_logo.svg" ,
    "res/txt/usage_stats.csv" ;
  .

okh:hasBoM
  a
    owl:ObjectProperty ,
    skos:Concept ;
  rdfs:label "has Bill of Materials"@en ;
  rdfs:comment "links to the corresponding Bill of Materials, which is a list or table of the parts required to build a component"@en ;
  dcam:domainIncludes okh:Module ;
  dcam:rangeIncludes ods:File ;
  vs:term_status "unstable" ;
  okhmeta:hasMetaTag
    okhmeta:DataTag ,
    okhmeta:PartsTag ;
  skos:example
    "bom.csv" ,
    "src/elec/bom.csv" ,
    "src/mech/bom.csv" ;
  .

okh:hasComponent
  a
    owl:ObjectProperty ,
    skos:Concept ;
  rdfs:label "has Component"@en ;
  rdfs:comment "Links to sub-components of the Module. In the case of that sub-component being an external Module, it has to refer to a snapshot of the RDF object representing that OKH Module. Each sub-component should also appear in the BoM."@en ;
  dcam:domainIncludes okh:Module ;
  dcam:rangeIncludes
    ods:FetchUrl ,
    okh:Component ;
  okhmeta:hasMetaTag okhmeta:PartsTag ;
  vaem:todo
    "TODO The two range value (see `dcam:rangeIncludes`) are an issue for the SHACL generator, because one is a class and the other a datatype, so it would have to be both OWL property types, but the SHACL generator (owl2shacl) can not handle that one (yet)" ,
    "TODO `rdfs:subPropertyOf schema:hasPart ;`? - Probably better suited for the OSH Ontology" ;
  .

okh:hasContributionGuide
  a
    owl:ObjectProperty ,
    skos:Concept ;
  rdfs:label "has contribution guide"@en ;
  rdfs:comment "links to the corresponding Contribution Guide"@en ;
  rdfs:subPropertyOf dcterms:instructionalMethod ;
  dcam:domainIncludes okh:Module ;
  dcam:rangeIncludes ods:File ;
  vs:term_status "unstable" ;
  okhmeta:hasMetaTag
    okhmeta:DocumentationTag ,
    okhmeta:ExtendedInfoTag ;
  .

okh:hasExport
  a
    owl:ObjectProperty ,
    skos:Concept ;
  rdfs:label "has exported file"@en ;
  rdfs:comment "Links to a file that was generated/exported from a source file of the project"@en ;
  dcam:domainIncludes okh:Component ;
  dcam:rangeIncludes ods:File ;
  rdfs:seeAlso
    okh:hasAuxiliary ,
    okh:hasSource ;
  vs:term_status "unstable" ;
  okhmeta:hasMetaTag
    okhmeta:BasicTag ,
    okhmeta:DataTag ;
  skos:example
    "gen/elec/converter/pcb.svg" ,
    "gen/elec/converter/schema.svg" ,
    "gen/mech/3D-parts/drawing.pdf" ,
    "gen/mech/3D-parts/drawing.png" ,
    "gen/mech/3D-parts/model2.stl" ,
    "gen/mech/3D-parts/part1.stp" ,
    "https://file-hosting-service.org/accounts/my_project/gen/elec/converter/pcb.svg" ,
    "https://my-orgs-server.org/projects/my_project/gen/mech/3D-parts/model2.stl" ,
    "https://my-projs-server.org/files/gen/mech/3D-parts/part1.stp" ;
  .

okh:hasImage
  a
    owl:ObjectProperty ,
    skos:Concept ;
  rdfs:label "has image"@en ;
  rdfs:comment "links to the corresponding Image"@en ;
  rdfs:subPropertyOf schema:image ;
  dcam:domainIncludes okh:Component ;
  dcam:rangeIncludes okh:Image ;
  vs:term_status "unstable" ;
  okhmeta:hasMetaTag okhmeta:BasicTag ;
  vaem:todo "TODO `rdfs:subPropertyOf foaf:depiction ;`? - This would probably be wrong, or at least misleading, because a project logo or a technical drawing of a part would fit for `okh:hasImage`, but not `foaf:depiction` -- Somehow related: `foaf:logo`, `doap:screenshot`" ;
  .

okh:hasManifestFile
  a
    owl:ObjectProperty ,
    skos:Concept ;
  rdfs:label "has manifest file"@en ;
  rdfs:comment "Links to the source TOML manifest file for (this) RDF data"@en ;
  rdfs:subPropertyOf dcterms:hasFormat ;
  dcam:domainIncludes okh:Dataset ;
  dcam:rangeIncludes okh:ManifestFile ;
  vs:term_status "unstable" ;
  okhmeta:hasMetaTag okhmeta:DataGatheringTag ;
  vaem:todo "TODO Comment out/remove this subject - This is now ODS territory, though there we use an ods:File now" ;
  .

okh:hasManufacturingInstructions
  a
    owl:ObjectProperty ,
    skos:Concept ;
  rdfs:label "has manufacturing instructions"@en ;
  rdfs:comment "Links to a file containing a manual/instructions of some kind, that explain how to manufacture the hardware."@en ;
  rdfs:subPropertyOf dcterms:instructionalMethod ;
  dcam:domainIncludes
    okh:Module ,
    okh:Part ;
  dcam:rangeIncludes ods:File ;
  vs:term_status "unstable" ;
  okhmeta:hasMetaTag
    okhmeta:DocumentationTag ,
    okhmeta:MakingTag ;
  skos:example "doc/assembly/main.md" ;
  .

okh:hasOuterDimensions
  a
    owl:ObjectProperty ,
    skos:Concept ;
  rdfs:label "outer dimensions"@en ;
  rdfs:comment "defined through width, depth and height in mm"@en ;
  rdfs:subPropertyOf
    dcterms:format ,
    okh:productionMetadata ;
  dcam:rangeIncludes okh:Dimensions ;
  vs:term_status "unstable" ;
  okhmeta:hasMetaTag okhmeta:PhysicalTag ;
  vaem:todo "TODO Maybe remove this and add hasProduct (1-*) instead, each one being of type <https://schema.org/Product>, which has width, height and depth also." ;
  .

okh:hasPublication
  a
    owl:ObjectProperty ,
    skos:Concept ;
  rdfs:label "has Publication"@en ;
  rdfs:comment "design files of this OSH module have been peer reviewed in the linked-to scientific publication"@en ;
  rdfs:subPropertyOf npg:hasPublication ;
  dcam:domainIncludes okh:Module ;
  dcam:rangeIncludes okh:Publication ;
  vs:term_status "unstable" ;
  okhmeta:hasMetaTag okhmeta:DevelopmentTag ;
  .

okh:hasReadme
  a
    owl:ObjectProperty ,
    skos:Concept ;
  rdfs:label "has ReadMe"@en ;
  rdfs:comment "repo-relative path (or absolute HTTP(S) URL) to to the corresponding ReadMe, which is the (human) entry-point into (the sources of) an OSH project"@en ;
  rdfs:subPropertyOf dcterms:instructionalMethod ;
  dcam:domainIncludes okh:Module ;
  dcam:rangeIncludes ods:File ;
  vs:term_status "unstable" ;
  okhmeta:hasMetaTag
    okhmeta:BasicTag ,
    okhmeta:DocumentationTag ;
  skos:example
    "README" ,
    "README-JP" ,
    "README-JP.md" ,
    "README.md" ,
    "README.txt" ;
  .

okh:hasSoftware
  a
    owl:ObjectProperty ,
    skos:Concept ;
  rdfs:label "has software"@en ;
  dcam:domainIncludes okh:Module ;
  dcam:rangeIncludes okh:Software ;
  vs:term_status "unstable" ;
  .

okh:hasSource
  a
    owl:ObjectProperty ,
    skos:Concept ;
  rdfs:label "has source file"@en ;
  rdfs:comment "Links to a file that forms part of the sources of the project; meaning, these are the primary files the designers and other contributors of the project are working on."@en ;
  dcam:domainIncludes okh:Component ;
  dcam:rangeIncludes ods:File ;
  rdfs:seeAlso
    okh:hasAuxiliary ,
    okh:hasExport ;
  vs:term_status "unstable" ;
  okhmeta:hasMetaTag
    okhmeta:BasicTag ,
    okhmeta:DataTag ;
  skos:example
    "https://my-orgs-server.org/projects/my_project/src/mech/3D-parts/model2.fcstd" ,
    "https://my-projs-server.org/files/src/elec/converter/proj1.kicad_pro" ,
    "https://repo-hosting-service.org/accounts/my_account/my_project/src/mech/3D-parts/part1.fcstd" ,
    "src/elec/converter/proj1.kicad_pro" ,
    "src/mech/3D-parts/model2.fcstd" ,
    "src/mech/3D-parts/part1.fcstd" ;
  .

okh:hasTag
  a
    owl:ObjectProperty ,
    skos:Concept ;
  rdfs:label "has tag"@en ;
  rdfs:comment """Links to a tag fit to describe the image.
The available tags are predefined,
see the [OKH image tags](http://w3id.org/oseg/ont/okhimg#tags);
there you will also read about the ability to define custom ones,
though you might also consider proposing a new common tag
[in an issue](https://github.com/iop-alliance/OpenKnowHow/issues/new).
An image can have multiple tags
and each tag can be used by multiple images
even within a single project."""@en ;
  rdfs:subPropertyOf schema:keywords ;
  dcam:domainIncludes okh:Image ;
  dcam:rangeIncludes schema:DefinedTerm ;
  vs:term_status "unstable" ;
  skos:example okhimg:tagArt ;
  .

okh:hasUserManual
  a
    owl:ObjectProperty ,
    skos:Concept ;
  rdfs:label "has user manual"@en ;
  rdfs:subPropertyOf dcterms:instructionalMethod ;
  dcam:domainIncludes okh:Module ;
  dcam:rangeIncludes ods:File ;
  vs:term_status "unstable" ;
  okhmeta:hasMetaTag okhmeta:DocumentationTag ;
  skos:example "doc/usr/main.md" ;
  .

okh:organization
  a
    owl:ObjectProperty ,
    skos:Concept ;
  rdfs:label "organization"@en ;
  rdfs:comment "organization of the licensor or that represents (some of) the contributors of the project"@en ;
  dcam:domainIncludes okh:Module ;
  dcam:rangeIncludes schema:Organization ;
  vs:term_status "unstable" ;
  okhmeta:hasMetaTag okhmeta:LegalTag ;
  .

okh:smallestToleranceClass
  a
    owl:ObjectProperty ,
    skos:Concept ;
  rdfs:label "smallest tolerance class"@en ;
  rdfs:comment "according to the ISO 286 standard"@en ;
  rdfs:subPropertyOf okh:productionMetadata ;
  dcam:domainIncludes okh:Part ;
  vs:term_status "unstable" ;
  okhmeta:hasMetaTag
    okhmeta:MakingTag ,
    okhmeta:PhysicalTag ;
  vaem:todo "TODO FIXME link! with rdfs:subPropertyOf"@en ;
  .

okh:technologyReadinessLevel
  a
    owl:ObjectProperty ,
    skos:Concept ;
  rdfs:label "Technology Readiness Level (TRL)"@en ;
  rdfs:comment "Indicates the development stage of the **hardware design** using the OTRL definitions; see the OTRL ontology."@en ;
  dcam:domainIncludes okh:Module ;
  dcam:rangeIncludes otrl:OTRL ;
  vs:term_status "unstable" ;
  owl:maxCardinality 1 ;
  okhmeta:hasMetaTag
    okhmeta:DevelopmentTag ,
    okhmeta:QualityTag ;
  skos:example
    otrl:OTRL1 ,
    otrl:OTRL2 ,
    otrl:OTRL3 ,
    otrl:OTRL4 ,
    otrl:OTRL5 ,
    otrl:OTRL6 ;
  .

okh:tsdc
  a
    owl:ObjectProperty ,
    skos:Concept ;
  rdfs:label "has related TsDC"@en ;
  rdfs:comment "Applicable _**T**echnology-**s**pecific **D**ocumentation **C**riteria_, according to DIN SPEC 3105-1, e.g. `tsdc:3DP`"@en ;
  dcam:domainIncludes okh:Component ;
  dcam:rangeIncludes tsdc:OHTsDC ;
  vs:term_status "unstable" ;
  okhmeta:hasMetaTag
    okhmeta:ExtendedInfoTag ,
    okhmeta:IdentificationTag ;
  skos:example
    tsdc:3DP ,
    tsdc:ASM ,
    tsdc:CMP ;
  .

okh:versionOf
  a
    owl:ObjectProperty ,
    skos:Concept ;
  rdfs:label "version of"@en ;
  rdfs:comment "connects specific versions of Modules with their versionless superclass"@en ;
  dcam:domainIncludes okh:Module ;
  dcam:rangeIncludes okh:Module ;
  vs:term_status "unstable" ;
  okhmeta:hasMetaTag
    okhmeta:HistoryTag ,
    okhmeta:IdentificationTag ;
  .

okh:attestation
  a
    owl:DatatypeProperty ,
    skos:Concept ;
  rdfs:label "attestation"@en ;
  rdfs:comment """A permanent URL to a valid attestation;
evidence of completeness and compliance to OSH principles,
for example from OSHWA, FSF, or DIN SPEC 3105.

Issuing conformity assessment bodies according to DIN SPEC 3105-2:

- [Open Hardware Observatory](https://en.oho.wiki/wiki/Request_certification_for_your_project)
- [Open Source Ecology Germany](https://gitlab.opensourceecology.de/verein/projekte/cab/CAB)

OSHWA:

- [OSHWA certification programme](https://certification.oshwa.org/)

FSF (computing only):

- [Hardware Devices that Support GNU/Linux](https://www.fsf.org/resources/hw)
"""@en ;
  dcam:domainIncludes okh:Module ;
  dcam:rangeIncludes ods:File ;
  vs:term_status "unstable" ;
  okhmeta:hasMetaTag
    okhmeta:DevelopmentTag ,
    okhmeta:QualityTag ;
  .

okh:cpcPatentClass
  a
    owl:DatatypeProperty ,
    skos:Concept ;
  rdfs:label "patent class"@en ;
  rdfs:comment """Cooperative Patent Classification identifier (CPC-ID)
of the International Patent Classification (IPC)
that describes best the field of technology of the OSH module.
To find the meaning of one,
or to find one fitting to your project,
please use this resource:
<https://worldwide.espacenet.com/classification>"""@en ;
  rdfs:subPropertyOf patent:classificationIPCInventive ;
  dcam:domainIncludes okh:Module ;
  dcam:rangeIncludes xsd:normalizedString ;
  vs:term_status "unstable" ;
  okhmeta:hasMetaTag
    okhmeta:BasicTag ,
    okhmeta:IdentificationTag ;
  skos:example "D03D 35/00" ;
  .

okh:depicts
  a
    owl:DatatypeProperty ,
    skos:Concept ;
  rdfs:comment """Human oriented description of what is visible in the image.
This matters for example:

- for visually impaired or blind people
- in case the image is not available
- to be able to put it as a caption next to the image"""@en ;
  rdfs:subPropertyOf
    dcterms:description ,
    foaf:depicts ,
    schema:abstract ;
  dcam:domainIncludes okh:Image ;
  dcam:rangeIncludes rdf:langString ;
  vs:term_status "unstable" ;
  okhmeta:hasMetaTag okhmeta:BasicTag ;
  skos:altLabel
    "has abstract"@en ,
    "has caption"@en ,
    "shows"@en ;
  skos:prefLabel "depicts"@en ;
  .

okh:depth
  a
    owl:DatatypeProperty ,
    skos:Concept ;
  rdfs:label "depth [mm]"@en ;
  rdfs:comment "The outer depth of the product"@en ;
  dcam:domainIncludes okh:Dimensions ;
  dcam:rangeIncludes xsd:float ;
  vs:term_status "unstable" ;
  owl:cardinality 1 ;
  okhmeta:hasMetaTag okhmeta:PhysicalTag ;
  sh:minExclusive 0 ;
  vaem:todo
    "TODO Define in the comment, whether this includes or excludes packaging"@en ,
    "TODO or should the range rather be int?"@en ;
  .

okh:documentationLanguage
  a
    owl:DatatypeProperty ,
    skos:Concept ;
  rdfs:label "documentation language"@en ;
  rdfs:comment """denotes the language of the documentation.
The concrete format is an IETF language tag
following the BCP 47 standard;
e.g. "en-GB\""""@en ;
  rdfs:subPropertyOf schema:inLanguage ;
  dcam:domainIncludes
    okh:Module ,
    okh:Part ,
    okh:Software ;
  vs:term_status "unstable" ;
  okhmeta:hasMetaTag okhmeta:DocumentationTag ;
  skos:example
    "de" ,
    "de-DE" ,
    "en" ,
    "en-GB" ,
    "en-US" ,
    "es" ;
  .

okh:doi
  a
    owl:DatatypeProperty ,
    skos:Concept ;
  rdfs:label "DOI"@en ;
  rdfs:comment "The digital object identifier (DOI) associated with the publication"@en ;
  rdfs:subPropertyOf npg:doi ;
  dcam:domainIncludes okh:Publication ;
  vs:term_status "unstable" ;
  okhmeta:hasMetaTag okhmeta:AcademicTag ;
  .

okh:function
  a
    owl:DatatypeProperty ,
    skos:Concept ;
  rdfs:label "functional description"@en ;
  rdfs:comment """What does the hardware actually do,
what problem does it solve,
for whom,
under which conditions etc.

If you wish that someone finds & uses your OSH -
specifically e.g. for solving a concrete medical issue -
include relevant keywords in this field.

Optional:
description of input, output and interfaces"""@en ;
  rdfs:subPropertyOf obo:BFO_0000016 ;
  dcam:domainIncludes okh:Module ;
  dcam:rangeIncludes rdf:langString ;
  vs:term_status "unstable" ;
  owl:cardinality 1 ;
  okhmeta:hasMetaTag okhmeta:BasicTag ;
  .

okh:hasMass
  a
    owl:DatatypeProperty ,
    skos:Concept ;
  rdfs:label "mass [g]"@en ;
  rdfs:comment "mass of the component in g"@en ;
  rdfs:subPropertyOf okh:productionMetadata ;
  dcam:rangeIncludes xsd:float ;
  vs:term_status "unstable" ;
  okhmeta:hasMetaTag okhmeta:PhysicalTag ;
  .

okh:height
  a
    owl:DatatypeProperty ,
    skos:Concept ;
  rdfs:label "height [mm]"@en ;
  rdfs:comment "The outer height of the product"@en ;
  dcam:domainIncludes okh:Dimensions ;
  dcam:rangeIncludes xsd:float ;
  vs:term_status "unstable" ;
  owl:cardinality 1 ;
  okhmeta:hasMetaTag okhmeta:PhysicalTag ;
  sh:minExclusive 0 ;
  vaem:todo
    "TODO Define in the comment, whether this includes or excludes packaging"@en ,
    "TODO or should the range rather be int?"@en ;
  .

okh:manufacturingProcess
  a
    owl:DatatypeProperty ,
    skos:Concept ;
  rdfs:label "manufacturing process"@en ;
  rdfs:subPropertyOf okh:productionMetadata ;
  vs:term_status "unstable" ;
  okhmeta:hasMetaTag okhmeta:MakingTag ;
  vaem:todo "TODO Needs more properties: comment and range"@en ;
  .

okh:material
  a
    owl:DatatypeProperty ,
    skos:Concept ;
  rdfs:label "material"@en ;
  rdfs:subPropertyOf okh:productionMetadata ;
  vs:term_status "unstable" ;
  okhmeta:hasMetaTag okhmeta:PhysicalTag ;
  vaem:todo "TODO Define the range of this property"@en ;
  .

okh:name
  a owl:DatatypeProperty ;
  rdfs:label "name"@en ;
  rdfs:comment "Working title of the OSH component"@en ;
  rdfs:subPropertyOf
    dcterms:title ,
    rdfs:label ;
  dcam:domainIncludes okh:Component ;
  vs:term_status "unstable" ;
  owl:cardinality 1 ;
  okhmeta:hasMetaTag
    okhmeta:BasicTag ,
    okhmeta:RequiredTag ;
  .

okh:normalizedManifestContent
  a
    owl:DatatypeProperty ,
    skos:Concept ;
  rdfs:label "has normalized manifest content"@en ;
  rdfs:comment """Points to a string literal containing the normalized (by the scraper)
content of the (TOML) manifest file, zlib compressed and base64 encoded.
We provide this,
so it can be used as a base for a manually curated manifest file for the project,
for a project that was scraped through a process that does not involve a manifest file,
like through an API of the hosting platform.
You should **not** use this as a data-source,
e.g. for searching the name of the project;
please use the RDF data for that!"""@en ;
  dcam:domainIncludes okh:Dataset ;
  dcam:rangeIncludes xsd:string ;
  vs:term_status "unstable" ;
  okhmeta:hasMetaTag okhmeta:DataGatheringTag ;
  .

okh:okhv
  a owl:DatatypeProperty ;
  rdfs:label "OKH version"@en ;
  rdfs:comment """The version of the OKH specification
the OSH projects metadata claims to follow.
Different version → different data fields in this file.
This describes the scraped-dataset,
so it refers to the OKH version the original meta-data at the source adheres to,
meaning the e.g. the TOML manifest manually created yb the project maintainers,
or the OKH v1 YAML manifest generated by the hosting platforms API.

The OKH version the final RDF data adheres to,
is specified by the OKH IRI it uses,
and simultaneously by the version defined in the owl:Ontology element
that is located at that IRI.

In general, this property will link to the same or an earlier version of the OKH spec,
compared to the version defined by the OKH namespace IRI
in the RDF version of a projects data."""@en ;
  rdfs:subPropertyOf schema:version ;
  dcam:domainIncludes ods:Dataset ;
  vs:term_status "unstable" ;
  owl:cardinality 1 ;
  .

okh:release
  a
    owl:DatatypeProperty ,
    skos:Concept ;
  rdfs:label "release"@en ;
  rdfs:comment "URL to release"@en ;
  dcam:domainIncludes
    okh:Module ,
    okh:Software ;
  dcam:rangeIncludes ods:FetchUrl ;
  vs:term_status "unstable" ;
  .

okh:standardID
  a
    owl:DatatypeProperty ,
    skos:Concept ;
  rdfs:label "document ID"@en ;
  rdfs:comment "document identifier for the technical standard"@en ;
  rdfs:subPropertyOf dcterms:identifier ;
  dcam:domainIncludes okh:Standard ;
  dcam:rangeIncludes xsd:normalizedString ;
  vs:term_status "unstable" ;
  okhmeta:hasMetaTag okhmeta:QualityTag ;
  .

okh:version
  a
    owl:DatatypeProperty ,
    skos:Concept ;
  rdfs:label "version"@en ;
  rdfs:comment "version of this Module, preferably following the [semantic versioning-scheme v2.0.0](https://semver.org/#semantic-versioning-200)"@en ;
  rdfs:subPropertyOf schema:version ;
  dcam:domainIncludes okh:Module ;
  vs:term_status "unstable" ;
  owl:cardinality 1 ;
  okhmeta:hasMetaTag
    okhmeta:HistoryTag ,
    okhmeta:IdentificationTag ;
  skos:example
    "0.0.1-24-g6a8a3a7" ,
    "1.0.0" ,
    "1.0.0-alpha" ,
    "1.0.0-alpha.1" ,
    "1.0.0-alpha.beta" ,
    "1.0.0-beta" ,
    "1.0.0-beta.11" ,
    "1.0.0-beta.2" ,
    "1.0.0-rc.1" ,
    "2.3.4" ,
    "6a8a3a7" ,
    "baf0e65d8d93e1b64e883dfd2ffc5b838a22ca25" ,
    "v0.3.1" ;
  .

okh:width
  a
    owl:DatatypeProperty ,
    skos:Concept ;
  rdfs:label "width [mm]"@en ;
  rdfs:comment "The outer width of the product"@en ;
  dcam:domainIncludes okh:Dimensions ;
  dcam:rangeIncludes xsd:float ;
  vs:term_status "unstable" ;
  owl:cardinality 1 ;
  okhmeta:hasMetaTag okhmeta:PhysicalTag ;
  sh:minExclusive 0 ;
  vaem:todo
    "TODO Define in the comment, whether this includes or excludes packaging"@en ,
    "TODO or should the range rather be int?"@en ;
  .

okh:functionalMetadata
  a
    rdf:Property ,
    skos:Concept ;
  rdfs:label "functionality metadata"@en ;
  rdfs:comment "Metadata addressing functionality, such as dimensions, material, weight, RPM,… (not standardized)"@en ;
  rdfs:subPropertyOf schema:value ;
  dcam:domainIncludes okh:Module ;
  vs:term_status "unstable" ;
  .

okh:productionMetadata
  a
    rdf:Property ,
    skos:Concept ;
  rdfs:label "production metadata"@en ;
  rdfs:comment "production-relevant metadata, such as material, manufacturing technology, outer dimensions, smallest tolerance, finest surface roughness"@en ;
  rdfs:subPropertyOf schema:value ;
  dcam:domainIncludes
    okh:Module ,
    okh:Part ;
  vs:term_status "unstable" ;
  okhmeta:hasMetaTag okhmeta:MakingTag ;
  vaem:todo "TODO This is somewhat superseded by okhmeta:MakingTag" ;
  .

